[Civl] Change failure preservation check (#1013)
The main goal of this PR is to change the implementation of the failure
preservation check. If L is a left mover and X is an arbitrary action,
the new formulation requires proving the validity of the following
condition:

wlp(L, gate(X)) ==> gate(X)

This implication can be stated informally as either of the following two
equivalent conditions.
- if it is impossible to get an execution of L from a state s leading
either to a failure of L or to a state violating gate(X), then s also
satisfies gate(X)
- if s fails gate(X), then there is a way to execute L from s leading
either to a failure of L or to a state that fails gate(X)

A useful aspect of the new formulation is that when the check fails,
blame can be assigned to a specific assertion in gate(X). This is
because the right side of the implication has a separate conjunct
corresponding to each assert.

It is a conjecture that if we check this new formulation of failure
preservation on a left mover, then the non-blocking check on a left
mover can be dropped. Intuitively, this new formulation appears to
capture the essential aspects of the old formulation of failure
preservation and the non-blocking check in one condition.

We would like the failure preservation check to have the desirable
property that if variables accessed in L are disjoint from those
accessed in gate(X), then the check is guaranteed to succeed. The
proposed failure preservation check does not have this property. But by
separately proving that L is nonblocking, we can reclaim this property
for the proposed check. Note that the nonblocking check is logically the
same as proving the validity wlp(L, false) ==> false.

Additionally:
- As a side effect of making the new formulation work on existing Civl
samples, add_to_pool annotations on assertions had to be propagated in
gate computation.
- To simplify gate computation, we now enforce that atomic actions
cannot refer to old(.).
- A small bug in pool instantiation was fixed.
- Error messages for mover checks were improved.
- 2PC proof based on inductive sequentialization is deleted because it
needed some porting and is going to be replaced anyway by an alternative
proof based on the new proof rule by @NamrathaG.
- Cooperation --> Nonblocking

Source/Concurrency/MoverCheck.cs
@@ -18,12 +18,12 @@ namespace Microsoft.Boogie
     HashSet<Tuple<Action, Action>> commutativityCheckerCache;
     HashSet<Tuple<Action, Action>> gatePreservationCheckerCache;
     HashSet<Tuple<Action, Action>> failurePreservationCheckerCache;
-    HashSet<Action> cooperationCheckerCache;
+    HashSet<Action> nonblockingCheckerCache;
 
     Dictionary<int, HashSet<Tuple<Action, Action>>> perLayerCommutativityCheckerCache;
     Dictionary<int, HashSet<Tuple<Action, Action>>> perLayerGatePreservationCheckerCache;
     Dictionary<int, HashSet<Tuple<Action, Action>>> perLayerFailurePreservationCheckerCache;
-    Dictionary<int, HashSet<Action>> perLayerCooperationCheckerCache;
+    Dictionary<int, HashSet<Action>> perLayerNonblockingCheckerCache;
 
     private MoverCheck(CivlTypeChecker civlTypeChecker, List<Declaration> decls)
     {
@@ -32,11 +32,11 @@ namespace Microsoft.Boogie
       this.commutativityCheckerCache = new HashSet<Tuple<Action, Action>>();
       this.gatePreservationCheckerCache = new HashSet<Tuple<Action, Action>>();
       this.failurePreservationCheckerCache = new HashSet<Tuple<Action, Action>>();
-      this.cooperationCheckerCache = new HashSet<Action>();
+      this.nonblockingCheckerCache = new HashSet<Action>();
       this.perLayerCommutativityCheckerCache = new Dictionary<int, HashSet<Tuple<Action, Action>>>();
       this.perLayerGatePreservationCheckerCache = new Dictionary<int, HashSet<Tuple<Action, Action>>>();
       this.perLayerFailurePreservationCheckerCache = new Dictionary<int, HashSet<Tuple<Action, Action>>>();
-      this.perLayerCooperationCheckerCache = new Dictionary<int, HashSet<Action>>();
+      this.perLayerNonblockingCheckerCache = new Dictionary<int, HashSet<Action>>();
     }
 
     private ConcurrencyOptions Options => civlTypeChecker.Options;
@@ -44,8 +44,6 @@ namespace Microsoft.Boogie
     public static void AddCheckers(CivlTypeChecker civlTypeChecker, List<Declaration> decls)
     {
       MoverCheck moverChecking = new MoverCheck(civlTypeChecker, decls);
-
-      // TODO: make enumeration of mover checks more efficient / elegant
 
       var regularMoverChecks =
         from first in civlTypeChecker.MoverActions
@@ -69,7 +67,7 @@ namespace Microsoft.Boogie
 
       foreach (var action in civlTypeChecker.MoverActions.Where(a => a.IsLeftMover))
       {
-        moverChecking.CreateCooperationChecker(action);
+        moverChecking.CreateNonblockingChecker(action);
       }
 
       /*
@@ -110,7 +108,7 @@ namespace Microsoft.Boogie
               layer = sequentialization.Layer,
               extraAssumptions = sequentialization.Preconditions(leftMover, subst).Select(assertCmd => assertCmd.Expr)
             };
-            moverChecking.CreateCooperationChecker(leftMover, moverCheckContext);
+            moverChecking.CreateNonblockingChecker(leftMover, moverCheckContext);
           }
         }
       }
@@ -121,7 +119,7 @@ namespace Microsoft.Boogie
       var availableVars = paramVars.Union(frame);
       return civlTypeChecker.linearTypeChecker.DisjointnessExprForEachDomain(availableVars)
         .Union(civlTypeChecker.linearTypeChecker.MapWellFormedExpressions(availableVars))
-        .Select(expr => new Requires(false, expr));
+        .Select(expr => RequiresHelper.Requires(expr));
     }
 
     private void AddChecker(string checkerName, List<Variable> inputs, List<Variable> outputs, List<Variable> locals,
@@ -199,16 +197,11 @@ namespace Microsoft.Boogie
         DisjointnessAndWellFormedRequires(
           first.FirstImpl.InParams.Union(second.SecondImpl.InParams)
             .Where(v => LinearTypeChecker.FindLinearKind(v) != LinearKind.LINEAR_OUT), frame).ToList();
-      foreach (AssertCmd assertCmd in first.FirstGate.Union(second.SecondGate))
-      {
-        requires.Add(new Requires(false, assertCmd.Expr));
-      }
+      requires.AddRange(first.FirstGate.Union(second.SecondGate).Select(assertCmd => RequiresHelper.Requires(assertCmd.Expr, assertCmd.Attributes)));
       if (moverCheckContext != null)
       {
         checkerName = $"CommutativityChecker_{first.Name}_{second.Name}_{moverCheckContext.layer}";
-        moverCheckContext.extraAssumptions.ForEach(extraAssumption => {
-          requires.Add(new Requires(false, extraAssumption));
-        });
+        requires.AddRange(moverCheckContext.extraAssumptions.Select(expr => RequiresHelper.Requires(expr)));
       }
 
       var transitionRelation = TransitionRelationComputation.Commutativity(civlTypeChecker, second, first, frame);
@@ -218,11 +211,10 @@ namespace Microsoft.Boogie
       IEnumerable<Expr> linearityAssumes = linearTypeChecker.DisjointnessExprForEachDomain(first.FirstImpl.OutParams.Union(secondInParamsFiltered)
         .Union(frame)).Union(linearTypeChecker.DisjointnessExprForEachDomain(first.FirstImpl.OutParams.Union(second.SecondImpl.OutParams)
           .Union(frame)));
-      // TODO: add further disjointness expressions?
-      AssertCmd commutativityCheck = CmdHelper.AssertCmd(
+      var commutativityCheck = CmdHelper.AssertCmd(
         first.tok,
         Expr.Imp(Expr.And(linearityAssumes), transitionRelation),
-        $"Commutativity check between {first.Name} and {second.Name} failed");
+        $"Commutativity check between {first.Name} @ {Location(first.ActionDecl.tok)} and {second.Name} @ {Location(second.ActionDecl.tok)} failed");
 
       List<Cmd> cmds = new List<Cmd>
       {
@@ -276,16 +268,11 @@ namespace Microsoft.Boogie
         DisjointnessAndWellFormedRequires(
           first.FirstImpl.InParams.Union(second.SecondImpl.InParams)
             .Where(v => LinearTypeChecker.FindLinearKind(v) != LinearKind.LINEAR_OUT), frame).ToList();
-      foreach (AssertCmd assertCmd in first.FirstGate.Union(second.SecondGate))
-      {
-        requires.Add(new Requires(false, assertCmd.Expr));
-      }
+      requires.AddRange(first.FirstGate.Union(second.SecondGate).Select(assertCmd => RequiresHelper.Requires(assertCmd.Expr, assertCmd.Attributes)));
       if (moverCheckContext != null)
       {
         checkerName = $"GatePreservationChecker_{first.Name}_{second.Name}_{moverCheckContext.layer}";
-        moverCheckContext.extraAssumptions.ForEach(extraAssumption => {
-          requires.Add(new Requires(false, extraAssumption));
-        });
+        requires.AddRange(moverCheckContext.extraAssumptions.Select(expr => RequiresHelper.Requires(expr)));
       }
 
       List<Variable> inputs = first.FirstImpl.InParams.Union(second.SecondImpl.InParams).ToList();
@@ -296,16 +283,9 @@ namespace Microsoft.Boogie
       IEnumerable<Expr> linearityAssumes =
         linearTypeChecker.DisjointnessExprForEachDomain(first.FirstImpl.InParams.Union(second.SecondImpl.OutParams)
           .Union(frame));
-      foreach (AssertCmd assertCmd in first.FirstGate)
-      {
-        cmds.Add(
-          CmdHelper.AssertCmd(
-            assertCmd.tok,
-            Expr.Imp(Expr.And(linearityAssumes), assertCmd.Expr),
-            $"Gate of {first.Name} not preserved by {second.Name}"
-          )
-        );
-      }
+      cmds.AddRange(first.FirstGate.Select(assertCmd =>
+        CmdHelper.AssertCmd(assertCmd.tok, Expr.Imp(Expr.And(linearityAssumes), assertCmd.Expr),
+            $"Gate of {first.Name} @ {Location(first.ActionDecl.tok)} not preserved by {second.Name} @ {Location(second.ActionDecl.tok)}")));
 
       AddChecker(checkerName, inputs, outputs, new List<Variable>(), requires, cmds);
     }
@@ -347,52 +327,42 @@ namespace Microsoft.Boogie
       var linearTypeChecker = civlTypeChecker.linearTypeChecker;
       List<Requires> requires = 
         DisjointnessAndWellFormedRequires(
-          first.FirstImpl.InParams.Union(second.SecondImpl.InParams)
-            .Where(v => LinearTypeChecker.FindLinearKind(v) != LinearKind.LINEAR_OUT), frame).ToList();
-      Expr firstNegatedGate = Expr.Not(Expr.And(first.FirstGate.Select(a => a.Expr)));
-      firstNegatedGate.Type = Type.Bool; // necessary?
-      requires.Add(new Requires(false, firstNegatedGate));
-      foreach (AssertCmd assertCmd in second.SecondGate)
-      {
-        requires.Add(new Requires(false, assertCmd.Expr));
-      }
+          first.FirstImpl.InParams.Union(second.SecondImpl.InParams).Where(v => LinearTypeChecker.FindLinearKind(v) != LinearKind.LINEAR_OUT), frame).ToList();
+      var wpreAssertCmds = Wlp.HoistAsserts(second.SecondImpl, first.FirstGate, Options);
+      requires.AddRange(wpreAssertCmds.Select(assertCmd => RequiresHelper.Requires(assertCmd.Expr, assertCmd.Attributes)));
+      requires.AddRange(second.SecondGate.Select(assertCmd => RequiresHelper.Requires(assertCmd.Expr, assertCmd.Attributes)));
+      
       if (moverCheckContext != null)
       {
         checkerName = $"FailurePreservationChecker_{first.Name}_{second.Name}_{moverCheckContext.layer}";
-        moverCheckContext.extraAssumptions.ForEach(extraAssumption => {
-          requires.Add(new Requires(false, extraAssumption));
-        });
+        requires.AddRange(moverCheckContext.extraAssumptions.Select(expr => RequiresHelper.Requires(expr)));
       }
 
+      var cmds = new List<Cmd>();
       IEnumerable<Expr> linearityAssumes =
-        linearTypeChecker.DisjointnessExprForEachDomain(first.FirstImpl.InParams.Union(second.SecondImpl.OutParams)
-          .Union(frame));
-      AssertCmd gateFailureCheck = CmdHelper.AssertCmd(
-        first.tok,
-        Expr.Imp(Expr.And(linearityAssumes), firstNegatedGate),
-        $"Gate failure of {first.Name} not preserved by {second.Name}");
+        linearTypeChecker.DisjointnessExprForEachDomain(first.FirstImpl.InParams.Union(second.SecondImpl.OutParams).Union(frame));
+      cmds.AddRange(linearityAssumes.Select(expr => new AssumeCmd(Token.NoToken, expr)));
 
       List<Variable> inputs = first.FirstImpl.InParams.Union(second.SecondImpl.InParams).ToList();
       List<Variable> outputs = first.FirstImpl.OutParams.Union(second.SecondImpl.OutParams).ToList();
-      var cmds = new List<Cmd>
-      {
-        ActionCallCmd(second, second.SecondImpl),
-        gateFailureCheck
-      };
+      cmds.AddRange(first.FirstGate.Select(assertCmd =>
+          CmdHelper.AssertCmd(assertCmd.tok, assertCmd.Expr,
+            $"Gate failure of {first.Name} @ {Location(first.ActionDecl.tok)} not preserved by {second.Name} @ {Location(second.ActionDecl.tok)}")
+      ));
 
       AddChecker(checkerName, inputs, outputs, new List<Variable>(), requires, cmds);
     }
 
-    private void CreateCooperationChecker(Action action) => CreateCooperationChecker(action, null);
+    private void CreateNonblockingChecker(Action action) => CreateNonblockingChecker(action, null);
 
-    private void CreateCooperationChecker(Action action, MoverCheckContext moverCheckContext)
+    private void CreateNonblockingChecker(Action action, MoverCheckContext moverCheckContext)
     {
       if (!action.HasAssumeCmd)
       {
         return;
       }
 
-      if (!cooperationCheckerCache.Add(action))
+      if (!nonblockingCheckerCache.Add(action))
       {
         return;
       }
@@ -400,17 +370,17 @@ namespace Microsoft.Boogie
       if (moverCheckContext != null)
       {
         var layer = moverCheckContext.layer;
-        if (!perLayerCooperationCheckerCache.ContainsKey(layer))
+        if (!perLayerNonblockingCheckerCache.ContainsKey(layer))
         {
-          perLayerCooperationCheckerCache[layer] = new HashSet<Action>();
+          perLayerNonblockingCheckerCache[layer] = new HashSet<Action>();
         }
-        if (!perLayerCooperationCheckerCache[layer].Add(action))
+        if (!perLayerNonblockingCheckerCache[layer].Add(action))
         {
           return;
         }
       }
 
-      string checkerName = $"CooperationChecker_{action.Name}";
+      string checkerName = $"NonblockingChecker_{action.Name}";
 
       Implementation impl = action.Impl;
       HashSet<Variable> frame = new HashSet<Variable>();
@@ -420,20 +390,22 @@ namespace Microsoft.Boogie
       List<Requires> requires =
         DisjointnessAndWellFormedRequires(impl.InParams.Where(v => LinearTypeChecker.FindLinearKind(v) != LinearKind.LINEAR_OUT),
           frame).ToList();
-      requires.AddRange(action.Gate.Select(assertCmd => new Requires(Token.NoToken, false, assertCmd.Expr, null, assertCmd.Attributes)));
+      requires.AddRange(action.Gate.Select(assertCmd => RequiresHelper.Requires(assertCmd.Expr, assertCmd.Attributes)));
       if (moverCheckContext != null)
       {
-        checkerName = $"CooperationChecker_{action.Name}_{moverCheckContext.layer}";
-        requires.AddRange(moverCheckContext.extraAssumptions.Select(expr => new Requires(false, expr)));
+        checkerName = $"NonblockingChecker_{action.Name}_{moverCheckContext.layer}";
+        requires.AddRange(moverCheckContext.extraAssumptions.Select(expr => RequiresHelper.Requires(expr)));
       }
 
-      AssertCmd cooperationCheck = CmdHelper.AssertCmd(
+      AssertCmd nonblockingCheck = CmdHelper.AssertCmd(
         action.tok,
-        TransitionRelationComputation.Cooperation(civlTypeChecker, action, frame),
-        $"Cooperation check for {action.Name} failed");
+        TransitionRelationComputation.Nonblocking(civlTypeChecker, action, frame),
+        $"Nonblocking check for {action.Name} failed");
 
       AddChecker(checkerName, new List<Variable>(impl.InParams), new List<Variable>(impl.OutParams),
-        new List<Variable>(), requires, new List<Cmd> { cooperationCheck });
+        new List<Variable>(), requires, new List<Cmd> { nonblockingCheck });
     }
+
+    private static string Location(IToken tok) => string.Format("{0}({1},{2})", tok.filename, tok.line, tok.col);
   }
 }
